Rewrite scheduler for forever

denotational/Logic.v
@@ -11,27 +11,213 @@ From ITree Require Import
 
 From CTree Require Import
      CTree
+     Interp.State
+     Trans
+     Equ
+     SBisim
+     CTreeDefinitions
      Core.Utils
      Interp.State.
 
 From ExtLib Require Import
      Maps
+     StateMonad
      FMapAList
      RelDec
      String
      Monad.
 
-From DSL Require Import Vectors.
+From Coinduction Require Import
+     coinduction rel tactics.
 
-Import MonadNotation.
+From DSL Require Import
+     Vectors
+     Utils
+     System.
+
+Import MonadNotation SBisimNotations.
 Local Open Scope monad_scope.
 Local Open Scope string_scope.
 
 Set Implicit Arguments.
 Set Contextual Implicit.
 
-(** Logic and ctrees *)
-Module Logic.
+Section HSimulation.
+  
+  Context {E F: Type -> Type} {X Y : Type}.
+  Program Definition sim(RL: rel (@label E) (@label F)): mon (ctree E X -> ctree F Y -> Prop) :=
+    {| body R t u :=
+      forall l t', trans l t t' -> exists l', RL l l' -> exists2 u', trans l' u u' & R t' u'
+    |}.
+  Next Obligation.
+    destruct (H0 _ _ H1).
+    exists x0. intros HL.
+    destruct (H2 HL).
+    exists x1; eauto.
+  Qed.
+End HSimulation.
+
+Module Shallow.
+  Module DS := DistributedSystems(DistrSystem).
+  Import DistrSystem Monad DS.
+
+  Variable (S: Type).
+
+  (** The linear temporal logic modality is encoded in the ctree,
+      the epistemic logic is reified to the Phi effect *)
+  Inductive Logic: Type -> Type :=
+  | Pred: (S -> Prop) -> Logic unit.
+
+  Notation ETL := (ctree Logic unit).
+  Notation ETL' := (ctree' Logic unit).
+  
+  Definition lift(p: S -> Prop): ETL :=
+    Vis (Pred p) (fun _ => Ret tt).  
+  
+  Definition next(p: ETL): ETL :=
+    TauV p.
+
+  CoFixpoint and_ltl(p q: ETL): ETL :=
+    match observe p, observe q with
+    | VisF (Pred p) k, VisF (Pred p') k' =>
+        Vis (Pred (fun s => p s /\ p' s))
+             (fun tt: unit => and_ltl (k tt) (k' tt))
+    | ChoiceF b n k, _ => (** distributive right *)
+        Choice b n (fun i: fin n => and_ltl (k i) q)
+    | _, ChoiceF b n k => (** distributive left *)
+        Choice b n (fun i: fin n => and_ltl p (k i))
+    | RetF _, _ => q
+    | _, RetF _ => p
+    end.
+
+  CoFixpoint or_ltl(p q: ETL): ETL :=
+    match observe p, observe q with
+    | VisF (Pred p) k, VisF (Pred p') k' =>
+        Vis (Pred (fun s => p s \/ p' s))
+             (fun tt: unit => or_ltl (k tt) (k' tt))
+    | ChoiceF b n k, _ => (** distributive right *)
+        Choice b n (fun i: fin n => and_ltl (k i) q)
+    | _, ChoiceF b n k => (** distributive left *)
+        Choice b n (fun i: fin n => and_ltl p (k i))
+    | RetF _, _ => q
+    | _, RetF _ => p
+    end.
+
+  Definition or_etl(p q: ETL): ETL :=
+    choiceV2 p q.
+                      
+  Definition until(p q: ETL): ETL :=
+    CTree.iter (fun _: unit =>
+                  choiceI2 
+                    (_ <- p;; Ret (inl tt))
+                    (_ <- q;; Ret (inr tt))) tt.
+
+  Definition forever(p: ETL): ETL :=
+    until p (lift (fun _ => False)).
+
+  Definition forever'(p: ETL): ETL :=
+    CTree.forever p.
+
+  (** They should be the same *)
+  Lemma forever_forever': forall p,
+      forever p ~ forever' p.
+  Proof.  
+    intros.
+    unfold sbisim.
+    coinduction ? ?.
+    unfold forever, forever', until.
+    rewrite Shallow.unfold_forever_.
+    rewrite unfold_iter; cbn.
+    cbn.
+    destruct (observe p) eqn:Hp.
+    cbn.
+    eauto; cbn.
+    eapply st_clo_bind.
+    __upto_bind_sbisim.
+    upto_bind_sbisim.
+    __upto_bind.
+    rewrite ctree_eta.
+    cbn.
+    destruct (observe p) eqn:Hp.
+    esplit.
+    apply_coinduction.
+    __coinduction_sbisim ? H.
+    __coinduction_equ ? ?.
+    esplit; [auto | cbn].
+    econstructor; cbn; intros.
+    - unfold forever, until in H.
+      rewrite unfold_iter in H.
+      cbn in H.
+      apply trans_bind_inv in H.
+      Print label.
+      inversion H.
+      destruct H.
+      Search trans.
+      eexists.
+  Admitted.
+  
+  (** Begin entailment relation on Vis states *)
+  Notation Sys R := (ctree (stateE S) R) (only parsing).
+  Notation Sys' R := (ctree' (stateE S) R) (only parsing).
+
+  Reserved Notation "a |-- b" (at level 40, left associativity).
+  Inductive entails_ {R} : Sys' R -> ETL' -> Prop :=
+  (** Visible state changes on the system match visible predicates of the logic *)
+  | PredPut: forall (p: S -> Prop) (h: S) (k: unit -> Sys R) (k': unit -> ETL),
+      p h ->
+      observe (k tt) |-- observe (k' tt) ->
+      VisF (Put h) k |-- VisF (Pred p) k'
+  (** My interpretation of 'choice' on the logic side is existential,
+      ie: I can chose which formula is satisfied by the current system.
+      This makes sense for the definition of 'p1 until p2' --
+      either p1 or p2 is satisfied but not both *)
+  | ChoiceLogic: forall n s k b,
+      (exists (i: fin n), s |-- observe (k i)) ->
+      s |-- ChoiceF b n k
+  (** Conversely, on the system side 'choice' is interpreted as 'all',
+      ie: all states of the system must be 'lawful'. *)
+  | ChoiceSystem: forall n f k b,
+      (forall (i: fin n), observe (k i) |-- f ) ->
+      ChoiceF b n k |-- f
+  (** Dont really care for 'Ret' *)
+  | RetLogic: forall t,    
+      t |-- RetF tt
+  | RetSystem: forall f r,
+      RetF r |-- f
+  where "a |-- b" := (entails_ a b).
+
+  Definition entails{R}(c: Sys R)(f: ETL): Prop :=
+    entails_ (observe c) (observe f).
+
+  Notation "a |= b" := (entails a b) (at level 40, left associativity).
+
+  Module St := Storage(DistrSystem).
+  Import St.
+
+  Definition foo : Sys unit :=
+    o <- load "a";;
+    let v := default o 0 in 
+    store "a" (v + 1).
+
+  Lemma foo_positive:
+    foo |= forever (lift (fun st => exists v, lookup "a" st = Some v /\ v > 0)).
+  Proof.
+    unfold foo, forever, until.
+    cbn.
+    Search CTree.iter.
+    Check unfold_iter.
+    rewrite unfold_iter.
+    unfold CTree.iter.
+    
+    rewrite bind_bind.
+    Search iter.
+    rewrite unfold_iter.
+    cbn.
+    econstructor.
+    un
+End Test.
+  
+Module ReturnLogic.
   CoInductive CTL s: Type :=
   | RetL: (s -> Prop) -> CTL s
   | NextL: CTL s -> CTL s
