denotational/Network.v
@@ -53,147 +53,83 @@ Module Network(S: Systems).
   Module Storage := Storage(S).
   Export Monads Storage Messaging S.
 
-  Notation InitSys n E R := (vec n (ctree E R)) (only parsing).
-  Notation Sys n E R := (vec n (Task n E R)) (only parsing).
-  Notation SysLeaf n R := (option (vec n (R * queue n))) (only parsing).
-  Notation SysTree n E R := (ctree E (SysLeaf n R)) (only parsing).
+  Notation Sys n E := (vec n (Task n E)) (only parsing).
 
-  Equations get_running{E A m n}(v: vec m (Task n E A))
-            (i: fin (num_running v)): (fin m * ctree E A * queue n) :=
-    get_running ((Running _ _) :: ts) (FS k) :=
-      let '(i, a, q) := get_running ts k in (FS i, a, q);
-    get_running ((Done _ _) :: ts) k :=
-      let '(i, a, q) := get_running ts k in (FS i, a, q);
-    get_running ((Blocked _ _) :: ts) k :=
-      let '(i, a, q) := get_running ts k in (FS i, a, q);
-    get_running ((Running a q) :: ts) F1 := (F1, a ,q).
-
-  (** Blocking processes might cause a deadlock, in which case we return 'None'
-      or `Some (vec n _)` (every agent returned)
-   *)
-  Equations schedule_network_0 {E A m n} (a: vec m (Task n E A))
-            (H: num_running a = 0): option (vec m (A * queue n)) :=
-    schedule_network_0 [] _ := Some [];
-    schedule_network_0 ((Done r q)::ts) _ :=
-      option_map (fun l => (r, q) :: l) (schedule_network_0 ts _);
-    schedule_network_0 ((Blocked _ _)::ts) _ := None.
-
-  Equations schedule_one{R: Type}{E: Type -> Type}{n: nat}
-            (schedule: Sys n (Net n +' E) R -> SysTree n E R)
-            (sys: Sys n (Net n +' E) R)
-            (r: fin (num_running sys)) : SysTree n E R :=
-    schedule_one schedule sys r with get_running sys r => {
-        schedule_one _ _ _ (i, a, q) with observe a => {
-          (** Returns a value *)
-          schedule_one _ _ _ _ (RetF v) :=
-            TauI (schedule (sys @ i := Done v q));
-        
+  Equations schedule_one{E: Type -> Type}{n: nat}
+            (schedule: Sys n (Net n +' E) -> ctree E (Sys n E))
+            (sys: Sys n (Net n +' E)) (r: fin n): ctree E (Sys n E) :=
+    schedule_one schedule sys r with sys $ r => {
+        schedule_one _ _ _ (Running a q) with observe a => {
           (** A previous choice, traverse it *)
           schedule_one _ _ _ _ (ChoiceF b n' k) :=
-            Choice b n' (fun i' => schedule (sys @ i := Running (k i') q));
-
+          Choice b n' (fun i' => schedule (sys @ r := Running (k i') q));
+          
           (** A network `send` effect, interpet it! *)
-          schedule_one _ _ _ _ (VisF (inl1 (Send m)) k) with (sys $ principal m)=>{
-            (** Deliver to running *)
-            schedule_one _ _ _ (i, _, _) _ (Running c q) :=
-              let msg' := {| principal := i; payload := payload m |} in
-              let sys' := sys @ i := Running (k tt) q in
-              let recp := principal m in
-              TauI (schedule (sys' @ recp := Running c (List.cons msg' q)));
-            
-            (** Deliver to blocked processes and unblock them *)
-            schedule_one _ _ _ (i, _, _) _ (Blocked c q) :=
-              let msg' := {| principal := i; payload := payload m |} in
-              let sys' := sys @ i := Running (k tt) q in
-              let recp := principal m in
-              TauI (schedule (sys' @ recp := Running c (List.cons msg' q)));
-            
-            (** Do not deliver to Done processes *)
-            schedule_one _ _ _ (i, _, _) _ (Done _ _) :=
-            TauI (schedule (sys @ i := Running (k tt) q))
-          };
+          schedule_one _ _ _ _ (VisF (inl1 (Send m)) k) :=
+          let msg' := {| principal := r; payload := payload m |} in
+          let sys' := sys @ r := Running (k tt) q in
+          match sys $ principal m with
+          | Running a' q' =>  
+              (** Deliver to running *)
+              TauI (schedule (sys' @ (principal m) := Running a' (List.cons msg' q')))
+          | Blocked kk => 
+              (** Deliver to blocked processes and unblock them *)
+              TauI (schedule (sys' @ (principal m) := Running (kk (Some msg')) List.nil))
+          end;
 
           (** Receive a message *)
-          schedule_one _ _ _ _ (VisF (inl1 Recv) k) with last q => {
-            (** Pop the msg from the end *)
-            schedule_one _ _ _ (i, _, _) _ (Some msg) :=
-              TauI (schedule (sys @ i := Running (k msg) (init q)));
-            (** Becomes blocked if no messages in q *)
-            schedule_one _ _ _ (i, _, _) _ None :=
-              TauI (schedule (sys @ i := Blocked a q))
-          };
+          schedule_one _ _ _ _ (VisF (inl1 Recv) k) :=
+            (** Check my inbox q *)
+            match last q with
+            | Some msg =>
+                (** Pop the msg from the end *)
+                TauI (schedule (sys @ r := Running (k (Some msg)) (init q)))
+            | None =>
+                (** Becomes blocked if no messages in q *)
+                TauI (schedule (sys @ r := Blocked k))
+            end;
 
           (** Broadcast a message to everyone *)
           schedule_one _ _ _ _ (VisF (inl1 (Broadcast b)) k) :=
-            let msg := {| principal := i; payload := b |} in
+            let msg := {| principal := r; payload := b |} in
             let sys' := map (fun a => match a with
-                                      | Running a q => Running a (List.cons msg q)
-                                      | Done a q => Done a q
-                                      | Blocked a q => Running a (List.cons msg q)
-                                      end) sys in 
-            TauI (schedule (sys' @ i := Running (k tt) q));
-              
-          (** Some other downstream effect *)
+                                   | Running a q => Running a (List.cons msg q)
+                                   | Blocked kk => Running (kk (Some msg)) List.nil
+                                   end) sys in 
+            TauI (schedule (sys' @ r := Running (k tt) q));
+          
+          (** Some other downstream effect, trigger *)
           schedule_one _ _ _ _ (VisF (inr1 e) k) :=
-            TauI (schedule (sys @ i := Running (trigger e >>= k) q))
-        }
-      }.
-  (** TODO: NON-det version 
-      sys'' <- mapT (fun a: list Msg * itree Net R =>
-      let (q', a') := a in
-      CTrees.choiceV2
-      (CTrees.Ret (msg :: q', a'))
-      (CTrees.Ret (q', a'))) sys';;
-      
-      CTrees.TauV (schedule sys'' done)
-   *)
+            TauI (schedule (sys @ r := Running (trigger e >>= k) q))
+        };
+        (** If the agent is blocked, it could timeout or stay blocked *)
+        schedule_one _ _ _ (Blocked k) :=
+          choiceI2
+            (schedule (sys @ r := Running (k None) List.nil))  (** Timeout *)
+            (schedule (sys @ r := Blocked k));                 (** Keep blocking *)
+    }.
 
-  Definition schedule_network{R: Type}{E}{n: nat}
-             (schedule: Sys n (Net n +' E) R -> SysTree n E R)
-             (sys: Sys n (Net n +' E) R): SysTree n E R :=
-    match num_running sys as n1 return
-          (num_running sys = n1 -> SysTree n E R) with
-    | 0 => fun Hnr: num_running sys = 0 =>
-             Ret (schedule_network_0 sys Hnr)
-    | S n1 => fun Hnr: num_running sys = S n1 =>
-                r <- choice false (num_running sys) ;;
-                schedule_one schedule sys r
-    end eq_refl.
-  
-  CoFixpoint schedule {R: Type}{E: Type -> Type}{n: nat} :=
-    @schedule_network R E n schedule.
-
-  Lemma rewrite_schedule: forall n R E (s: Sys n (Net n +' E) R),
-      schedule s ≅ schedule_network schedule s.
-  Proof.
-    intros.
-    __step_equ.
-    eauto.
-  Qed.
+  CoFixpoint schedule{E}{n: nat}(sys: Sys n (Net n +' E)): ctree E (Sys n E) :=
+    r <- choice false n ;;
+    schedule_one schedule sys r.
 
   Typeclasses eauto := 6.
 
   Transparent schedule.
   Transparent schedule_one.
-  Transparent schedule_network_0.
-  Transparent get_running.
   Transparent vector_replace.
 
   (** Evaluates Net *)
-  Definition run_network{E R n} (s: InitSys n (Net n +' E) R): SysTree n E R :=
+  Definition run_network{E n} (s: vec n (ctree (Net n +' E) void)): ctree E (Sys n E) :=
     schedule (Vector.map (fun it => Running it List.nil) s).
 
-  #[global] Instance sbisim_clos_network_goal{n E R}:
-    Proper (sbisim ==> eq ==> sbisim) (fun h ts => @run_network E R (S n) (h :: ts)).
+  #[global] Instance sbisim_clos_network_goal{n E}:
+    Proper (sbisim ==> eq ==> sbisim) (fun h ts => @run_network E (S n) (h :: ts)).
   Proof.
-    unfold Proper, respectful, run_network.
+    unfold Proper, respectful.
     intros x y Hxy nx ny Hn.
+    unfold run_network.
     cbn.
-    remember (map (fun it : ctree (Net (S n) +' E) R => Running it Datatypes.nil) nx) as netx.
-    remember (map (fun it : ctree (Net (S n) +' E) R => Running it Datatypes.nil) ny) as nety.
-    eapply transitivity with (y:=schedule_one schedule (Running x List.nil :: netx) (F1)); cbn.
-    - desobs x.
-      cbn.
   Admitted.
 
 End Network.
